more reorganization around sorted_wrt

src/HOL/Data_Structures/Sorted_Less.thy
@@ -11,39 +11,29 @@ hide_const sorted
 text \<open>Is a list sorted without duplicates, i.e., wrt @{text"<"}?
 Could go into theory List under a name like @{term sorted_less}.\<close>
 
-fun sorted :: "'a::linorder list \<Rightarrow> bool" where
-"sorted [] = True" |
-"sorted [x] = True" |
-"sorted (x#y#zs) = (x < y \<and> sorted(y#zs))"
-
-lemma sorted_Cons_iff:
-  "sorted(x # xs) = (sorted xs \<and> (\<forall>y \<in> set xs. x < y))"
-by(induction xs rule: sorted.induct) auto
-
-lemma sorted_snoc_iff:
-  "sorted(xs @ [x]) = (sorted xs \<and> (\<forall>y \<in> set xs. y < x))"
-by(induction xs rule: sorted.induct) auto
+abbreviation sorted :: "'a::linorder list \<Rightarrow> bool" where
+"sorted \<equiv> sorted_wrt (op <)"
 
 lemma sorted_cons: "sorted (x#xs) \<Longrightarrow> sorted xs"
-by(simp add: sorted_Cons_iff)
+by(simp add: sorted_wrt_Cons)
 
 lemma sorted_cons': "ASSUMPTION (sorted (x#xs)) \<Longrightarrow> sorted xs"
 by(rule ASSUMPTION_D [THEN sorted_cons])
 
 lemma sorted_snoc: "sorted (xs @ [y]) \<Longrightarrow> sorted xs"
-by(simp add: sorted_snoc_iff)
+by(simp add: sorted_wrt_append)
 
 lemma sorted_snoc': "ASSUMPTION (sorted (xs @ [y])) \<Longrightarrow> sorted xs"
 by(rule ASSUMPTION_D [THEN sorted_snoc])
 
 lemma sorted_mid_iff:
   "sorted(xs @ y # ys) = (sorted(xs @ [y]) \<and> sorted(y # ys))"
-by(induction xs rule: sorted.induct) auto
+by(fastforce simp add: sorted_wrt_Cons sorted_wrt_append)
 
 lemma sorted_mid_iff2:
   "sorted(x # xs @ y # ys) =
   (sorted(x # xs) \<and> x < y \<and> sorted(xs @ [y]) \<and> sorted(y # ys))"
-by(induction xs rule: sorted.induct) auto
+by(fastforce simp add: sorted_wrt_Cons sorted_wrt_append)
 
 lemma sorted_mid_iff': "NO_MATCH [] ys \<Longrightarrow>
   sorted(xs @ y # ys) = (sorted(xs @ [y]) \<and> sorted(y # ys))"
@@ -55,10 +45,10 @@ text\<open>Splay trees need two additional @{const sorted} lemmas:\<close>
 
 lemma sorted_snoc_le:
   "ASSUMPTION(sorted(xs @ [x])) \<Longrightarrow> x \<le> y \<Longrightarrow> sorted (xs @ [y])"
-by (auto simp add: Sorted_Less.sorted_snoc_iff ASSUMPTION_def)
+by (auto simp add: sorted_wrt_append ASSUMPTION_def)
 
 lemma sorted_Cons_le:
   "ASSUMPTION(sorted(x # xs)) \<Longrightarrow> y \<le> x \<Longrightarrow> sorted (y # xs)"
-by (auto simp add: Sorted_Less.sorted_Cons_iff ASSUMPTION_def)
+by (auto simp add: sorted_wrt_Cons ASSUMPTION_def)
 
 end
